Sketches of some basic proofs about timer driver

pancake/serial/serialPanDrvProofScript.sml
@@ -3,6 +3,45 @@ open serialPanDrvTheory panSemTheory;
 
 val _ = new_theory "serialPanDrvProof"
 
+Definition uart_device_oracle_def:
+  uart_device_oracle = ARB (* TODO (eventually) *)
+End
 
-    
+Definition uart_init_state_def:
+  uart_init_state ck be mem memaddrs ffi =
+  <| locals := FEMPTY;
+     code := FEMPTY |++ serialProg;
+     eshapes := FEMPTY; (* TODO: should there be something here? *)
+     memory := mem;
+     memaddrs := memaddrs;
+     clock := ck;
+     be := be;
+     ffi := ffi
+    |> 
+End
+
+Theorem uart_drv_getcharFun_no_break:
+  ∀ck be mem memaddrs ffi res s.
+    (evaluate (Call Tail (Label (strlit "uart_drv_getchar")) [],
+               uart_init_state ck be mem memaddrs ffi) = (res,s)) ∧
+    preconditions (* TODO *) ⇒
+    res ≠ SOME Break
+Proof
+  (* TODO *)
+QED
+        
+Theorem uart_drv_getcharFun_no_break:
+  ∀ck be mem memaddrs ffi res s.
+    (evaluate (Call Tail (Label (strlit "uart_drv_getchar")) [],
+               uart_init_state ck be mem memaddrs ffi) = (res,s)) ∧
+    preconditions (* TODO *) ⇒
+    res ≠ SOME Error
+Proof
+  rpt strip_tac >>
+  fs[Once evaluate_def,uart_init_state_def,serialProg_def,
+     uart_drv_getcharFun_def, uart_drv_putcharFun_def] >>
+  fs[Once eval_def,flookup_fupdate_list,ALOOKUP_def] >>
+  (* TODO *)
+QED
+
 val _ = export_theory();
